Improved the Decidable lemmas, shortened the List-decideability lemmas, and added DecidableSasn.

Java/src/CaseStudies/List.v
@@ -1,5 +1,5 @@
-Require Import Program  Heap ProtocolLogic AssertionLogic OperationalSemantics SpecLogic Util IsMarshallable.
-Require Import MapInterface MapFacts List.
+Require Import Program  Heap ProtocolLogic AssertionLogic OperationalSemantics SpecLogic Util Decidable.
+Require Import MapInterface MapFacts List RelationClasses Setoid.
 Require Import SepAlg SepAlgInsts ILInsts ILogic ILEmbed ILEmbedTac ILQuantTac OpenILogic
                SepAlgMap UUSepAlg Open Subst Stack Lang SemCmd HeapArr ST SemCmdRules BILogic BILInsts Rel.
 
@@ -13,194 +13,42 @@ Fixpoint Node_list (p : val) (xs : list sval) : asn :=
 .
 
 Definition List_rep (p : val) (xs : list sval) : asn :=
-  Exists head, pointsto p "head" head ** Node_list head xs.
+  Exists head, Node_list head xs ** pointsto p "head" head.
 
 Local Existing Instance DecSval.
 
-Local Transparent ILPre_Ops.
-Local Transparent ILPreFrm_pred.
-Local Transparent EmbedSasnPureOp.
-Local Transparent EmbedILFunOp.
-Local Transparent EmbedAsnPropOp.
-Local Transparent ILPre_Ops.
-Local Transparent EmbedILPreDropOp.
-Local Transparent EmbedILPreOp.
-Local Transparent MapSepAlgOps.
-Local Transparent ILFun_Ops.
-Local Transparent EmbedILFunDropOp.
-Local Transparent EmbedILFunOp.
-Local Transparent SepAlgOps_prod.
-
-Local Transparent EmbedILPreDropOp.
-Local Transparent EmbedILFunDropOp.
-Local Transparent EmbedPSasnPropOp.
-Local Transparent EmbedAsnPropOp.
-Local Transparent BILOperatorsPSasn.
-Local Transparent BILFun_Ops.
-Local Transparent BILOperatorsAsn.
-Local Transparent ILOpsSAsn.
-Local Transparent EmbedAsnPropOp.
-Local Transparent EmbedILPreDropOp.
-
-Lemma Node_list_decidable (p : val) (xs : list sval) : DecidableAsn (`Node_list `p `xs).
+Lemma Node_list_decidable (p : val) (xs : list sval) : DecidableAsn (Node_list p xs).
 Proof.
-  unfold liftn, lift, var_expr; simpl.
   generalize dependent p.
   induction xs.
-  * intros p s Pr n h.
-    destruct (dec_eq p null).
-    left; apply e.
-    right; intro Hfail; auto.
-  * intros p s Pr n h.
-    destruct (dec_eq (val_to_ptr p) pnull) as [Hnull | Hnotnull]; [
-      right; intro Hfail; destruct Hfail as [p' [h1 [h2 [Hh [HNodeList [h3 [h4 [Hh2 [[HPval _] _]]]]]]]]]; simpl in HPval; auto |].
-    destruct p; try (right; intro Hfail; destruct Hfail as [p' [h1 [h2 [Hh [HNodeList [h3 [h4 [Hh2 [[HPval _] _]]]]]]]]]; simpl in HPval; apply HPval; reflexivity).
-  
-    destruct (In_dec (get_heap_ptr h) (p, "val")) as [Hinval | Hnotinval]; [destruct Hinval as [val Hinval] |].
-    destruct (dec_eq a val); [subst |].
-    destruct (In_dec (get_heap_ptr h) (p, "next")) as [Hinnext | Hnotinnext]; [destruct Hinnext as  [next Hinnext] |].
-    specialize (IHxs next s Pr n (mkheap (remove (p, "val") (remove (p, "next") (get_heap_ptr h))) (get_heap_arr h))).
-    destruct IHxs.
-    - (* success, we can do the pointstos and the recursion *)
-      left. 
-      exists next. (* pick the value we found for next *)
-      
-      (* Pick the heap minus p.next and p.val for the recursion *)
-      exists (mkheap (remove (p, "val") (remove (p, "next") (get_heap_ptr h))) (get_heap_arr h)).
-      exists (mkheap (add (p, "val") val (add (p, "next") next (empty _))) (empty _)).
-      assert (sa_mul (mkheap (remove (p, "val") (remove (p, "next") (get_heap_ptr h))) (get_heap_arr h))
-                     (mkheap (add (p, "val") val (add (p, "next") next (empty Stack.val))) (empty Stack.val)) h). {
-        apply split_heap; simpl; [| apply uusa_unit; apply empty_1 ].
-        apply sa_mulC. apply sa_mul_swapL; [| assumption ]. apply sa_mul_swapL; [| assumption]. apply sa_mulC. apply uusa_unit; apply empty_1.
-      }
-      exists H0.
-      split; [assumption |]. (* use the induction hypothethis to deal with the recursion *)
-      
-      (* Pick the relevant subheaps for p.next and p.val *)
-      exists (mkheap (add (p, "val") val (empty _)) (empty _)).
-      exists (mkheap (add (p, "next") next (empty _)) (empty _)).
-      assert (sa_mul (mkheap (add (p, "val") val (empty Stack.val)) (empty Stack.val))
-                     (mkheap (add (p, "next") next (empty Stack.val)) (empty Stack.val))
-                     (mkheap (add (p, "val") val (add (p, "next") next (empty Stack.val))) (empty Stack.val))). {
-         apply split_heap; simpl; [| apply uusa_unit; apply empty_1].
-         eapply sa_mul_add. apply sa_mulC. apply uusa_unit; apply empty_1.
-         intro Hfail.
-         apply add_neq_in_iff in Hfail; [apply empty_in_iff in Hfail; apply Hfail |].
-         intro Hfail'. inversion Hfail'; subst. inversion H6; subst. unfold "===", _eq in H5. 
-         inversion H8; subst. inversion H10; subst. inversion H12; subst.
-      }
-      exists H1.
-      (* Use the singleton heaps to solve the pointstos *)
-      split; simpl; (split; [assumption |]); exists (empty _); apply uusa_unit; apply empty_1.
-    - (* failure, we cannot do the recursion *)
-      right; intro Hfail; apply H.
-      destruct Hfail as [? Hfail].
-      assert (next = x). {
-        (* Use pointsto p.next x and MapsTo p.next next to unify x and next *)
-        destruct Hfail as [h1 [h2 [Hh [HNodeList [h3 [h4 [Hh2 [_ [_ HP]]]]]]]]]; simpl in HP.
-        destruct HP as [h3_ptr HP].
-        eapply sa_mul_mapstoL in HP; [| apply add_1; reflexivity ].
-        apply sa_mulC in Hh2; apply isolate_heap_ptr in Hh2; eapply sa_mul_mapstoL in Hh2; [| apply HP].
-        apply sa_mulC in Hh; apply isolate_heap_ptr in Hh; eapply sa_mul_mapstoL in Hh; [| apply Hh2].
-        destruct Hh as [Hh _].
-        apply find_mapsto_iff in Hh; apply find_mapsto_iff in Hinnext.
-        unfold field in Hh; unfold field in Hinnext (* Ay ay ay *).
-        rewrite Hinnext in Hh. inversion Hh; reflexivity.
-      }
-      rewrite H0 in *.
-      destruct Hfail as [h1 [h2 [Hh [HNodeList Hfail]]]].
-      (* Solve using the induction hypothethis *)
-      solve_model HNodeList; [unfold rel | congruence].
-      (* Pick what must be the taken out to form the subheap h1 *)
-      exists (mkheap (remove (p, "val") (remove (p, "next") (get_heap_ptr h2))) (get_heap_arr h2)).
-      apply split_heap; simpl; [| apply Hh].
-      (* Use what we know from the pointsto to show that we can remove p.val and p.next from both sides *)
-      destruct Hfail as [h3 [h4 [Hh2 [[_ Hval] [_ Hnext]]]]].
-      simpl in Hval; destruct Hval as [? Hval]; eapply sa_mul_mapstoL in Hval; [| apply add_1; reflexivity]; destruct Hval as [Hval _]; clear x0.
-      simpl in Hnext; destruct Hnext as [? Hnext]; eapply sa_mul_mapstoL in Hnext; [| apply add_1; reflexivity]; destruct Hnext as [Hnext _]; clear x0.
-      apply sa_mulC; apply sa_mul_remove; [ apply sa_mul_remove; [apply sa_mulC; apply Hh |] |].
-      (* Show that p.next and p.val are infact in h2, not in h1 *)
-      + apply sa_mulC in Hh2. apply isolate_heap_ptr in Hh2; eapply sa_mul_inL in Hh2; [| exists x; eassumption].
-        apply sa_mulC in Hh; apply isolate_heap_ptr in Hh; eapply sa_mul_inL in Hh; [ apply Hh | apply Hh2 ]. 
-      + apply isolate_heap_ptr in Hh2; eapply sa_mul_inL in Hh2; [| exists val; eassumption].
-        apply sa_mulC in Hh; apply isolate_heap_ptr in Hh; eapply sa_mul_inL in Hh; [ apply Hh | apply Hh2 ].
-    - (* failure, there is no next-pointer *)
-      right; intro Hfail; apply Hnotinnext.
-      destruct Hfail as [p' [h1 [h2 [Hh [HNodeList [h3 [h4 [Hh2 [ _ [_ Hnext]]]]]]]]]].
-      simpl in Hnext; destruct Hnext as [? Hnext]; eapply sa_mul_mapstoL in Hnext; [| apply add_1; reflexivity]; destruct Hnext as [Hnext _]; clear x.
-      apply sa_mulC in Hh2; apply isolate_heap_ptr in Hh2; eapply sa_mul_inL in Hh2; [| exists p'; eassumption ].
-      apply sa_mulC in Hh; apply isolate_heap_ptr in Hh; eapply sa_mul_inL in Hh; [| apply Hh2]; apply Hh.
-    - (* failure, the value in the list is different to the value in the heap *)
-      right; intro Hfail; apply n0.
-      destruct Hfail as [_ [h1 [h2 [Hh [_ [h3 [h4 [Hh2 [[_ Hval] _]]]]]]]]].
-      simpl in Hval; destruct Hval as [? Hval]; eapply sa_mul_mapstoL in Hval; [| apply add_1; reflexivity]; destruct Hval as [Hval _]; clear x.
-      apply isolate_heap_ptr in Hh2; eapply sa_mul_mapstoL in Hh2; [| eassumption ].
-      apply sa_mulC in Hh; apply isolate_heap_ptr in Hh; eapply sa_mul_mapstoL in Hh; [| apply Hh2].
-      destruct Hh as [Hmapsto _].
-      apply find_mapsto_iff in Hinval; apply find_mapsto_iff in Hmapsto.
-      unfold field in Hinval; unfold field in Hmapsto (* Ay ay ay *).
-      rewrite Hinval in Hmapsto. inversion Hmapsto; reflexivity. 
-    - (* failure, there is no value-pointer *)
-      right; intro Hfail; apply Hnotinval.
-      destruct Hfail as [_ [h1 [h2 [Hh [_ [h3 [h4 [Hh2 [[_ Hval] _]]]]]]]]].
-      simpl in Hval; destruct Hval as [? Hval]; eapply sa_mul_mapstoL in Hval; [| apply add_1; reflexivity]; destruct Hval as [Hval _]; clear x.
-      apply isolate_heap_ptr in Hh2; eapply sa_mul_inL in Hh2; [| exists a; eassumption ].
-      apply sa_mulC in Hh; apply isolate_heap_ptr in Hh; eapply sa_mul_inL in Hh; [| apply Hh2]; apply Hh.
+  * intros p Pr n h.
+    destruct (dec_eq p null); [ left; apply e | right; intro Hfail; auto ].
+  * intro p.
+    assert (forall (p' : sval), DecidableAsn (@sepSP asn _ (Node_list p' xs) (pointsto p "val" a))).
+      intros p'. specialize (IHxs p').
+      apply pointsto_decidable_2 with (v := p) (f := "val") (e := a) in IHxs.
+      exact IHxs.
+    apply decidable_existsI with (p := p) (f := "next") in H.
+    unfold Node_list; fold Node_list.
+    setoid_rewrite <- sepSPA.
+    exact H.
 Qed.
 
-Lemma List_rep_decidable (p : val) (xs : list sval) : DecidableAsn (`List_rep `p `xs).
+Lemma List_rep_decidable (p : val) (xs : list sval) : DecidableAsn (List_rep p xs).
+Proof.  
+  unfold List_rep.
+  apply decidable_existsI.
+  intro p'; apply Node_list_decidable.
+Qed.
+
+Lemma List_rep_decidable_val (p : val) (xs : list sval) : DecidableSasn (`List_rep `p `xs).
 Proof.
-  intros s Pr n h.
-  unfold liftn, lift; simpl.
-  destruct (dec_eq (val_to_ptr p) pnull) as [Hnull | Hnotnull]; [
-    right; intro Hfail; destruct Hfail as [p' [h1 [h2 [Hh [[Hhead _] _]]]]]; simpl in Hhead; auto |].
-  destruct p;
-    try (right; intro Hfail; destruct Hfail as [p' [h1 [h2 [Hh [[Hhead _] _]]]]]; simpl in Hhead; apply Hhead; reflexivity).
-  
-  destruct (In_dec (get_heap_ptr h) (p, "head")) as [[head Hin] | Hnotin].
-  remember (mkheap (remove (p, "head") (get_heap_ptr h)) (get_heap_arr h)) as h'.
-  destruct (Node_list_decidable head xs s Pr n h').
-  - (* success, the node starts at `head` *)
-    left.
-    exists head.
-    exists (mkheap (add (p, "head") head (empty _)) (empty _)).
-    exists (mkheap (remove (p, "head") (get_heap_ptr h)) (get_heap_arr h)).
-    assert (sa_mul (mkheap (add (p, "head") head (empty val)) (empty val))
-                   (mkheap (remove (p, "head") (get_heap_ptr h)) (get_heap_arr h)) h). {
-	  apply split_heap; simpl; [| apply sa_mulC; apply uusa_unit; apply empty_1 ].
-	  eapply sa_mul_swapL; [| assumption].
-	  apply sa_mulC; apply uusa_unit; apply empty_1.
-	}
-	exists H0.
-	unfold liftn, lift in H; simpl in H. rewrite Heqh' in H.
-	split; [| assumption].
-	simpl. split; [apply Hnotnull |].
-	exists (empty _); apply uusa_unit; apply empty_1.
-  - (* failure, the list doesn't start at `head` *)
-    right. intro Hfail; apply H; clear H.
-    destruct Hfail as [head' Hfail].
-    assert (head = head'). {
-      destruct Hfail as [h1 [h2 [Hh [[_ Hhead] _]]]].
-      simpl in Hhead; destruct Hhead as [? Hhead]; eapply sa_mul_mapstoL in Hhead; [| apply add_1; reflexivity]; destruct Hhead as [Hhead _]; clear x.
-      apply isolate_heap_ptr in Hh; eapply sa_mul_mapstoL in Hh; [| apply Hhead].
-      destruct Hh as [Hh _].
-      apply find_mapsto_iff in Hh; apply find_mapsto_iff in Hin.
-      unfold field in Hh; unfold field in Hin (* Ay ay ay *).
-      rewrite Hh in Hin. inversion Hin; reflexivity.
-    }
-    rewrite <- H in *; clear H.
-    unfold liftn, lift; simpl; rewrite Heqh'.
-    destruct Hfail as [h1 [h2 [Hh [[_ Hhead] HNodeList]]]].
-    simpl in Hhead; destruct Hhead as [? Hhead]; eapply sa_mul_mapstoL in Hhead; [| apply add_1; reflexivity]; destruct Hhead as [Hhead _]; clear x.
-    solve_model HNodeList; [| congruence].
-    unfold rel.
-    exists (mkheap (remove (p, "head") (get_heap_ptr h1)) (get_heap_arr h1)).
-    apply split_heap; simpl; apply sa_mulC; [| apply Hh].
-    apply sa_mul_remove; [apply Hh |].
-    eapply sa_mul_inL; [apply Hh | exists head; apply Hhead].
-  - (* failure, p.head isn't in the heap *)
-    right. intro Hfail; apply Hnotin; clear Hnotin.
-    destruct Hfail as [head' [h1 [h2 [Hh [[_ Hhead] _]]]]].
-    simpl in Hhead; destruct Hhead as [? Hhead]; eapply sa_mul_mapstoL in Hhead; [| apply add_1; reflexivity]; destruct Hhead as [Hhead _]; clear x.
-    apply isolate_heap_ptr in Hh; eapply sa_mul_inL in Hh; [| exists head'; eassumption]; apply Hh.
+  intros s. unfold liftn, lift; simpl.
+  apply List_rep_decidable.
+Qed.
+
+Lemma List_rep_decidable_var (p : var) (xs : list sval) : DecidableSasn (`List_rep p/V `xs).
+Proof.
+  intros s. unfold liftn, lift, var_expr; simpl.
+  apply List_rep_decidable.
 Qed.
