Java/src/Logic/Decidable.v
@@ -29,20 +29,19 @@ Local Transparent ILOpsSAsn.
 
 Local Existing Instance DecSval.
 
-Lemma pointsto_decidable (v : var) (f : field) (e : expr) :
-  (* @lentails sasn _ (@ltrue sasn _) *) (DecidableAsn (`pointsto v/V `f e)).
+Lemma pointsto_decidable (v : val) (f : field) (e : val) :
+  (DecidableAsn (pointsto v f e)).
 Proof.
-  intros (*_ _ _ _ _*) s Pr n h.
-  destruct (dec_eq (s v) null) as [Hnull | Hnotnull]; [
+  intros Pr n h; simpl.
+  destruct (dec_eq v null) as [Hnull | Hnotnull]; [
     unfold var_expr; simpl; right; intro Hfail; destruct Hfail as [Hfail _]; rewrite Hnull in Hfail; auto |].
-  remember (s v) as ptr; destruct ptr;
-    try (unfold var_expr; simpl; right; intro Hfail; destruct Hfail as [Hfail _]; rewrite <- Heqptr in Hfail; apply Hfail; reflexivity).
+  destruct v;
+    try (unfold var_expr; simpl; right; intro Hfail; destruct Hfail as [Hfail _]; apply Hfail; reflexivity).
   assert (p <> pnull) as Hnotpnull by (intro Hfail; apply Hnotnull; unfold null; rewrite Hfail; reflexivity).
-  unfold liftn, lift, var_expr; simpl.
-  rewrite <- Heqptr in *; simpl.
+  
   destruct (In_dec (get_heap_ptr h) (p, f)) as [Hin | Hnotin].
   destruct Hin as [k Hmapsto].
-  destruct (dec_eq k (e s)) as [Heq | Hneq]; [ subst |].
+  destruct (dec_eq k e) as [Heq | Hneq]; [ subst |].
   - left; split; [assumption |].
     exists (remove (p, f) (get_heap_ptr h)).
     apply sa_mul_swapL; [apply sa_mulC; apply uusa_unit; apply empty_1 | assumption].
@@ -53,49 +52,46 @@ Proof.
     destruct Hfail as [[Hfail _] | [_ Hfail]].
     + apply find_mapsto_iff in Hfail. rewrite add_eq_o in Hfail; [| reflexivity].
       inversion Hfail; reflexivity.
-    + exfalso; apply Hfail; exists (e s).
+    + exfalso; apply Hfail; exists e.
       apply add_1; reflexivity.
   - right. intros Hfail; destruct Hfail as [_ Hfail].
     apply Hnotin.
     unfold subheap in Hfail; destruct Hfail as [? Hfail].
-    exists (e s).
+    exists e.
     eapply sa_mul_mapstoL; [apply Hfail |].
     apply add_1; reflexivity.
 Qed.
 
-Lemma pointsto_decidable_2 (v : var) (f : field) (e : expr) (Q : sasn) :
-  DecidableAsn Q -> DecidableAsn (Q ** `pointsto v/V `f e).
+Lemma pointsto_decidable_2 (v : val) (f : field) (e : val) (Q : asn) :
+  DecidableAsn Q -> DecidableAsn (Q ** pointsto v f e).
 Proof.
   unfold DecidableAsn; simpl.
-  intros (* _ _ _ _ *) H s Pr n h.
+  intros H Pr n h; simpl.
   
-  destruct (dec_eq (s v) null) as [Hnull | Hnotnull]; [
+  destruct (dec_eq v null) as [Hnull | Hnotnull]; [
     unfold var_expr; right; intro Hfail; destruct Hfail as [h1 [h2 [Hh [_ [HP _]]]]]; simpl in HP; rewrite Hnull in HP; auto |].
-  remember (s v) as ptr; destruct ptr;
-    try (unfold var_expr; right; intro Hfail; destruct Hfail as [h1 [h2 [Hh [_ [HP _]]]]]; simpl in HP; rewrite <- Heqptr in HP; apply HP; reflexivity).
-  assert (p <> pnull) as Hnotpnull by (intro Hfail; apply Hnotnull; unfold null; rewrite Hfail; reflexivity).
+  destruct v;
+    try (unfold var_expr; right; intro Hfail; destruct Hfail as [h1 [h2 [Hh [_ [HP _]]]]]; simpl in HP; apply HP; reflexivity).
+  assert (p <> pnull) as Hnotpnull by (intro Hfail; apply Hnotnull; rewrite Hfail; reflexivity).
   
-  specialize (H s Pr n (mkheap (remove (p, f) (get_heap_ptr h)) (get_heap_arr h))).
+  specialize (H Pr n (mkheap (remove (p, f) (get_heap_ptr h)) (get_heap_arr h))).
   destruct H as [HQ | notHQ].
   * destruct (In_dec (get_heap_ptr h) (p, f)) as [Hin | Hnotin].
     destruct Hin as [k Hmapsto]. 
-    destruct (dec_eq k (e s)) as [Heq | Hneq]; [ subst |].
-    - left.
+    destruct (dec_eq k e) as [Heq | Hneq]; [ subst |].
+    - left; simpl.
       exists (mkheap (remove (p, f) (get_heap_ptr h)) (get_heap_arr h)).
-      exists (mkheap (add (p, f) (e s) (empty _)) (empty _)).
+      exists (mkheap (add (p, f) e (empty _)) (empty _)).
       assert (sa_mul (mkheap (remove (p, f) (get_heap_ptr h)) (get_heap_arr h)) 
-                     (mkheap (add (p, f) (e s) (empty val)) (empty val)) h) by (
+                     (mkheap (add (p, f) e (empty val)) (empty val)) h) by (
         apply split_heap; simpl; [apply sa_mulC; apply sa_mul_swapL; [apply sa_mulC; apply uusa_unit; apply empty_1 | apply Hmapsto] |
       	  						  apply uusa_unit; apply empty_1]).
       exists H.
       split; [ apply HQ |].
-      unfold liftn, lift, var_expr; simpl.
-      rewrite <- Heqptr; simpl. split; [ apply Hnotpnull |].
+      simpl. split; [ apply Hnotpnull |].
       exists (empty _); apply uusa_unit; apply empty_1.
-    - right; intro Hfail. destruct Hfail as [h1 [h2 [Hh [_ [_ HP]]]]].
-      unfold liftn, lift, var_expr in HP; simpl in HP.
-      destruct HP as [? HP].
-      rewrite <- Heqptr in HP; simpl in HP.
+    - right; simpl; intro Hfail. destruct Hfail as [h1 [h2 [Hh [_ [_ HP]]]]].
+      destruct HP as [? HP]; simpl in HP.
       eapply sa_mul_mapstoL in HP; [| apply add_1; reflexivity ].
       apply sa_mulC in Hh. apply isolate_heap_ptr in Hh. eapply sa_mul_mapstoL in Hh; [| apply HP].
       destruct Hh as [Hh _].
@@ -104,9 +100,8 @@ Proof.
       apply Hneq; inversion Hmapsto; reflexivity.
     - right. intro Hfail. destruct Hfail as [h1 [h2 [Hh [_ [_ HP]]]]].
       unfold liftn, lift, var_expr in HP; simpl in HP.
-      apply Hnotin; exists (e s).
-      destruct HP as [? HP].
-      rewrite <- Heqptr in HP; simpl in HP.
+      apply Hnotin; exists e.
+      destruct HP as [? HP]; simpl in HP.
       eapply sa_mul_mapstoL in HP; [| apply add_1; reflexivity ].
       apply sa_mulC in Hh. apply isolate_heap_ptr in Hh. eapply sa_mul_mapstoL in Hh; [| apply HP].
       apply Hh.
@@ -119,10 +114,9 @@ Proof.
 	assert (~ In (p, f) (get_heap_ptr h1)). {
 	  intro Hfail.
 	  unfold liftn, lift, var_expr in HP; simpl in HP.
-	  destruct HP as [_ [? HP]].
-	  rewrite <- Heqptr in HP; simpl in HP.
+	  destruct HP as [_ [? HP]]; simpl in HP.
 	  eapply sa_mul_mapstoL in HP; [| apply add_1; reflexivity ].
-	  apply isolate_heap_ptr in Hh; apply sa_mulC in Hh; eapply sa_mul_inL in Hh; [| exists (e s); apply HP].
+	  apply isolate_heap_ptr in Hh; apply sa_mulC in Hh; eapply sa_mul_inL in Hh; [| exists e; apply HP].
 	  destruct Hh as [Hh _].
 	  apply Hh; apply Hfail.
     }
@@ -130,11 +124,73 @@ Proof.
     eapply sa_mul_remove; [ apply sa_mulC; apply Hh | apply H ].
 Qed.
 
-Lemma exists_decidable {A : Type} (P : A -> sasn) (a : A) : DecidableAsn( P a ) -> DecidableAsn( Exists a, P a). 
+Lemma decidable_existsI (p : val) (f : field) (P : sval -> asn) : 
+  (forall a, DecidableAsn (P a)) -> DecidableAsn ( @lexists asn _ _ (fun a => (P a)  ** pointsto p f a)). 
+Proof.
+  intros H Pr n h; simpl.
+  destruct (dec_eq p pnull) as [Hnull | Hnotnull]; [
+    right; intro Hfail; destruct Hfail as [p' [h1 [h2 [Hh [_ [Hhead _]]]]]]; simpl in Hhead; rewrite Hnull in Hhead; auto |].
+  destruct p;
+    try (right; intro Hfail; destruct Hfail as [p' [h1 [h2 [Hh [_ [Hhead _]]]]]]; simpl in Hhead; apply Hhead; reflexivity).
+  assert (p <> pnull) as Hnotpnull by congruence.
+  
+  destruct (In_dec (get_heap_ptr h) (p, f)) as [[val Hin] | Hnotin].
+  remember (mkheap (remove (p, f) (get_heap_ptr h)) (get_heap_arr h)) as h'.
+  destruct (H val Pr n h').
+  - (* success, P holds for val *)
+    left.
+    exists val.
+    exists (mkheap (remove (p, f) (get_heap_ptr h)) (get_heap_arr h)).
+    exists (mkheap (add (p, f) val (empty _)) (empty _)).
+    assert (sa_mul (mkheap (remove (p, f) (get_heap_ptr h)) (get_heap_arr h)) 
+                   (mkheap (add (p, f) val (empty _)) (empty _)) h). {
+	  apply split_heap; simpl; [| apply uusa_unit; apply empty_1 ].
+	  apply sa_mulC; eapply sa_mul_swapL; [| assumption].
+	  apply sa_mulC; apply uusa_unit; apply empty_1.
+	}
+	exists H1.
+	rewrite Heqh' in H0.
+	split; [assumption |].
+	simpl. split; [apply Hnotpnull |].
+	exists (empty _); apply uusa_unit; apply empty_1.
+  - (* failure, P doesn't hold for val *)
+    right.
+    intro Hfail; apply H0; clear H0.
+    destruct Hfail as [val' [h1 [h2 [Hh [HP [_ Hval]]]]]].
+    simpl in Hval; destruct Hval as [? Hval]; eapply sa_mul_mapstoL in Hval; [| apply add_1; reflexivity]; destruct Hval as [Hval _]; clear x.
+    assert (val = val'). {
+      apply sa_mulC in Hh; apply isolate_heap_ptr in Hh; eapply sa_mul_mapstoL in Hh; [| eassumption].
+      destruct Hh as [Hh _].
+      apply find_mapsto_iff in Hh; apply find_mapsto_iff in Hin.
+      rewrite Hh in Hin. inversion Hin; reflexivity.
+    }
+    rewrite H0; clear H0.
+    solve_model HP; [| congruence ].
+    unfold rel. rewrite Heqh'.
+    exists (mkheap (remove (p, f) (get_heap_ptr h2)) (get_heap_arr h2)).
+    apply split_heap; simpl; [| apply Hh].
+    apply sa_mulC; apply sa_mul_remove; [ apply sa_mulC; apply Hh |].
+    eapply sa_mul_mapstoL; [ eapply sa_mulC; apply Hh | apply Hval ].
+  - (* failure, there is no p.f in the heap *)
+    right.
+    intro Hfail; apply Hnotin; clear Hnotin.
+    destruct Hfail as [head' [h1 [h2 [Hh [_ [_ Hval]]]]]].
+    simpl in Hval; destruct Hval as [? Hval]; eapply sa_mul_mapstoL in Hval; [| apply add_1; reflexivity]; destruct Hval as [Hval _]; clear x.
+    apply sa_mulC in Hh; apply isolate_heap_ptr in Hh; eapply sa_mul_inL in Hh; [| exists head'; eassumption]; apply Hh.
+Qed.
+
+Global Instance DecidableAsn_m : Proper (lequiv ==> iff) DecidableAsn.
+Proof.
+  intros x y Hentails; split; (intros H Pr n h; destruct (H Pr n h); [
+    left; apply Hentails; apply H0 | 
+    right; intro Hfail; apply H0; apply Hentails; apply Hfail]).
+Defined.
+
+Lemma exists_decidable {A : Type} (P : A -> asn) (a : A) : DecidableAsn( P a ) -> DecidableAsn( Exists a, P a). 
 Proof.
   intro H.
-  intros s Pr n h.
-  specialize (H s Pr n h).
+  intros Pr n h.
+  specialize (H Pr n h).
   destruct H as [H | notH].
   left.
   exists a; assumption.
